Started adapting examples to variable-y syntax

src/sep/Locals.v
@@ -1,6 +1,7 @@
 Require Import Ascii Bool String List.
 Require Import Word Memory Expr SepExpr SymEval SepIL Env Prover SymEval IL SymIL.
 Require Import sep.Array.
+Require Import Allocated.
 
 Set Implicit Arguments.
 
@@ -8,8 +9,9 @@ Definition vals := string -> W.
 
 Definition toArray (ns : list string) (vs : vals) : list W := map vs ns.
 
-Definition locals (ns : list string) (vs : vals) (p : W) : HProp :=
-  ([| NoDup ns |] * array (toArray ns vs) p)%Sep.
+Definition locals (ns : list string) (vs : vals) (avail : nat) (p : W) : HProp :=
+  ([| NoDup ns |] * array (toArray ns vs) p
+    * Ex n, [| (n >= avail)%nat |] * ((p ^+ $(length ns * 4)) =?> n))%Sep.
 
 Definition ascii_eq (a1 a2 : ascii) : bool :=
   let (b1, c1, d1, e1, f1, g1, h1, i1) := a1 in
@@ -213,7 +215,7 @@ Section parametric.
   Definition sym_read (summ : Prover.(Facts)) (args : list (expr types)) (p : expr types)
     : option (expr types) :=
     match args with
-      | ns :: vs :: p' :: nil =>
+      | ns :: vs :: _ :: p' :: nil =>
         match deref p, listIn ns with
           | Some (base, offset), Some ns =>
             if Prover.(Prove) summ (Equal wordT p' base)
@@ -230,7 +232,7 @@ Section parametric.
   Definition sym_write (summ : Prover.(Facts)) (args : list (expr types)) (p v : expr types)
     : option (list (expr types)) :=
     match args with
-      | ns :: vs :: p' :: nil =>
+      | ns :: vs :: avail :: p' :: nil =>
         match deref p, listIn ns with
           | Some (base, offset), Some ns' =>
             if Prover.(Prove) summ (Equal wordT p' base)
@@ -238,7 +240,7 @@ Section parametric.
                      | None => None
                      | Some nm => Some (ns
                        :: Func updF (vs :: Const (types := types) (t := stringT) nm :: v :: nil)
-                       :: p' :: nil)
+                       :: avail :: p' :: nil)
                    end
               else None
           | _, _ => None
@@ -258,7 +260,7 @@ Section correctness.
   Definition types0 := types types'.
 
   Definition ssig : SEP.predicate types0 pcT stT.
-    refine (SEP.PSig _ _ _ (listStringT :: valsT :: wordT :: nil) _).
+    refine (SEP.PSig _ _ _ (listStringT :: valsT :: natT :: wordT :: nil) _).
     exact locals.
   Defined.
 
@@ -383,7 +385,7 @@ Section correctness.
     end.
   Proof.
     simpl; intuition.
-    do 4 (destruct args; simpl in *; intuition; try discriminate).
+    do 5 (destruct args; simpl in *; intuition; try discriminate).
     generalize (deref_correct uvars vars pe); destr idtac (deref pe); intro Hderef.
     destruct p0.
     generalize (listIn_correct uvars vars e); destr idtac (listIn e); intro HlistIn.
@@ -411,24 +413,31 @@ Section correctness.
     specialize (Hderef _ _ _ H1 (refl_equal _)).
     destruct Hderef as [ ? [ ] ].
     subst.
-    case_eq (exprD funcs uvars vars e1 wordT); [ intros ? Heq' | intro Heq' ]; rewrite Heq' in *; try tauto.
+    unfold types0 in H2.
+    unfold types0 in H1.
+    case_eq (exprD funcs uvars vars e1 natT); [ intros ? Heq' | intro Heq' ]; rewrite Heq' in *; try tauto.
+    case_eq (exprD funcs uvars vars e2 wordT); [ intros ? Heq'' | intro Heq'' ]; rewrite Heq'' in *; try tauto.
     rewrite H in H4.
     specialize (H4 (ex_intro _ _ (refl_equal _))).
     hnf in H4; simpl in H4.
-    rewrite Heq' in H4.
+    rewrite Heq'' in H4.
     rewrite H in H4.
     subst.
     Require Import PropXTac.
     apply simplify_fwd in H2.
     destruct H2 as [ ? [ ? [ ? [ ] ] ] ].
-    simpl simplify in *.
-    destruct H3.
-    apply simplify_bwd in H4.
-    generalize (split_semp _ _ _ H2 H5); intro; subst.
-    specialize (smem_read_correct' _ _ _ _ (i := natToW n) H4); intro Hsmem.
+    destruct H3 as [ ? [ ? [ ? [ ] ] ] ].
+    destruct H4 as [ ? [ ? [ ? [ ? [ ] ] ] ] ].
+    simpl simplify in H2, H3, H5, H4, H7.
+    destruct H5, H7.
+    apply simplify_bwd in H6.
+    generalize (split_semp _ _ _ H3 H9); intro; subst.
+    specialize (smem_read_correct' _ _ _ _ (i := natToW n) H6); intro Hsmem.
     rewrite natToW_times4.
     rewrite wmult_comm.
     unfold natToW in *.
+    erewrite split_smem_get_word; eauto.
+    left.
     rewrite Hsmem.
     f_equal.
 
@@ -443,7 +452,7 @@ Section correctness.
 
     unfold Array.sel.
     apply array_selN.
-    apply array_bound in H4.
+    apply array_bound in H6.
     rewrite wordToNat_natToWord_idempotent; auto.
     apply nth_error_Some_length in Heq.
 
@@ -462,7 +471,7 @@ Section correctness.
     apply Nlt_in.
     repeat rewrite wordToN_nat.
     repeat rewrite Nat2N.id.
-    apply array_bound in H4.
+    apply array_bound in H6.
     rewrite length_toArray in *.
     repeat rewrite wordToNat_natToWord_idempotent.
     eapply nth_error_Some_length; eauto.
@@ -500,7 +509,7 @@ Section correctness.
     end.
   Proof.
     simpl; intuition.
-    do 4 (destruct args; simpl in *; intuition; try discriminate).
+    do 5 (destruct args; simpl in *; intuition; try discriminate).
     generalize (deref_correct uvars vars pe); destr idtac (deref pe); intro Hderef.
     destruct p0.
     specialize (Hderef _ _ _ H1 (refl_equal _)).
@@ -528,27 +537,36 @@ Section correctness.
     rewrite HlistIn.
     simpl exprD.
     destruct (exprD funcs uvars vars e0 valsT); try tauto.
-    rewrite H2.
     unfold Provable in H6.
     simpl in H6.
     rewrite H4 in H6.
-    destruct (exprD funcs uvars vars e1 wordT); try tauto.
+    destruct (exprD funcs uvars vars e1 natT); try tauto.
+    destruct (exprD funcs uvars vars e2 wordT); try tauto.
+    rewrite H2.
     specialize (H6 (ex_intro _ _ (refl_equal _))); subst.
     apply simplify_fwd in H3.
     destruct H3 as [ ? [ ? [ ? [ ] ] ] ].
-    simpl simplify in *.
-    destruct H3.
-    apply simplify_bwd in H5.
-    eapply smem_write_correct' in H5.
-    destruct H5 as [ ? [ ] ].
+    destruct H3 as [ ? [ ? [ ? [ ] ] ] ].
+    destruct H5 as [ ? [ ? [ ? [ ? [ ] ] ] ] ].
+    simpl in H, H3, H6, H7, H5, H8.
+    destruct H6, H8.
+    apply simplify_bwd in H7.
+    eapply smem_write_correct' in H7.
+    destruct H7 as [ ? [ ] ].
     rewrite natToW_times4.
     rewrite wmult_comm.
-    generalize (split_semp _ _ _ H H6); intro; subst.
-    rewrite H5.
+    generalize (split_semp _ _ _ H3 H10); intro; subst.
+    generalize (split_semp _ _ _ H5 H11); intro; subst.
+    eapply split_set_word in H7.
+    destruct H7.
+    destruct H; subst.
+    rewrite H13.
     unfold locals.
     apply simplify_bwd.
+    exists x7; exists x6.
+    repeat split; auto.
     exists smem_emp.
-    exists x2.
+    exists x7.
     simpl; intuition.
     apply split_a_semp_a.
     reflexivity.
@@ -586,24 +604,37 @@ Section correctness.
       eapply nth_error_In; eauto.
     Qed.
 
-    unfold Array.upd in H7.
-    rewrite wordToNat_natToWord_idempotent in H7.
-    erewrite array_updN in H7; eauto.
+    unfold Array.upd in H12.
+    rewrite wordToNat_natToWord_idempotent in H12.
+    erewrite array_updN in H12; eauto.
     apply nth_error_Some_length in Heq.
-    apply array_bound in H7.
+    apply array_bound in H12.
     Require Import Arrays.
-    rewrite updN_length in H7.
-    rewrite length_toArray in H7.
+    rewrite updN_length in H12.
+    rewrite length_toArray in H12.
     apply Nlt_in.
     rewrite Nat2N.id.
     rewrite Npow2_nat.
     omega.
 
+    exists x4.
+    exists smem_emp.
+    exists x6.
+    split.
+    apply split_a_semp_a.
+    split.
+    simpl.
+    split.
+    auto.
+    reflexivity.
+    assumption.
+    destruct H; auto.
+
     rewrite length_toArray.
     apply Nlt_in.
     repeat rewrite wordToN_nat.
     repeat rewrite Nat2N.id.
-    apply array_bound in H5.
+    apply array_bound in H7.
     rewrite length_toArray in *.
     repeat rewrite wordToNat_natToWord_idempotent.
     eapply nth_error_Some_length; eauto.
@@ -648,3 +679,97 @@ Definition pack : MEVAL.MemEvaluatorPackage types_r (tvType 0) (tvType 1) (tvTyp
       (tvType 0) (tvType 1)))
   (fun ts => MemEvaluator _)
   (fun ts fs ps => MemEvaluator_correct _ _).
+
+
+(** * Some additional helpful theorems *)
+
+Theorem sel_upd_eq : forall vs nm v nm',
+  nm = nm'
+  -> sel (upd vs nm v) nm' = v.
+  unfold sel, upd; intros; subst; rewrite string_eq_true; reflexivity.
+Qed.
+
+Theorem sel_upd_ne : forall vs nm v nm',
+  nm <> nm'
+  -> sel (upd vs nm v) nm' = sel vs nm'.
+  unfold sel, upd; intros; subst; rewrite string_eq_false; auto.
+Qed.
+
+Require Import PropX.
+
+Theorem locals_weaken : forall ns vs avail avail' p,
+  (avail' <= avail)%nat
+  -> locals ns vs avail p ===> locals ns vs avail' p.
+  Ltac simp := cbv beta; unfold In.
+  intros; intro; hnf; intros.
+  unfold locals, starB, star.
+  apply Imply_I.
+  eapply Exists_E.
+  eauto.
+  simp; intros.
+  eapply Exists_E.
+  apply Env.
+  simp.
+  eauto.
+  simp; intros.
+  eapply Exists_E.
+  eapply And_E1.
+  eapply And_E2.
+  apply Env.
+  simp; eauto.
+  simp; intros.
+  eapply Exists_E.
+  apply Env.
+  simp; eauto.
+  simp; intro.
+  eapply Exists_E.
+  unfold exB, ex; simp.
+  eapply And_E2.
+  eapply And_E2.
+  apply Env; simp; eauto.
+  simp; intro.
+  eapply Exists_E.
+  apply Env; simp; eauto.
+  simp; intro.
+  eapply Exists_E.
+  apply Env; simp; eauto.
+  simp; intro.
+  apply Exists_I with B.
+  apply Exists_I with B0.
+  unfold exB, ex; simp.
+  apply And_I.
+  eapply And_E1.
+  apply Env; simp; eauto 10.
+  apply And_I.
+  apply Exists_I with B1.
+  apply Exists_I with B2.
+  apply And_I.
+  eapply And_E1.
+  apply Env; simp; eauto 10.
+  eapply And_E2.
+  apply Env; simp; eauto 10.
+  apply Exists_I with B3.
+  apply Exists_I with B4.
+  apply Exists_I with B5.
+  apply And_I.
+  eapply And_E1.
+  apply Env; simp; eauto.
+  apply And_I.
+  apply And_I.
+  apply Inj_E with (B3 >= avail)%nat.
+  eapply And_E1.
+  eapply And_E1.
+  eapply And_E2.
+  unfold injB, inj; simp.
+  apply Env; simp; eauto.
+  intro.
+  apply Inj_I.
+  omega.
+  unfold injB, inj.
+  eapply And_E2.
+  eapply And_E1.
+  eapply And_E2.
+  apply Env; simp; eauto.
+  do 2 eapply And_E2.
+  apply Env; simp; eauto.
+Qed.
