src/Arrays.v
@@ -1,4 +1,4 @@
-Require Import Word PropX PropXTac Memory SepIL Programming.
+Require Import Word PropX PropXTac Memory SepIL IL.
 
 Require Import sep.Array.
 
@@ -59,13 +59,13 @@ Hint Resolve bound_N_nat.
 
 Lemma sel_selN : forall ls (a : nat),
   (a < pow2 32)%nat
-  -> sel ls a = selN ls a.
+  -> sel ls (natToW a) = selN ls a.
   unfold sel; intros; rewrite wordToNat_natToWord_idempotent; auto.
 Qed.
 
 Lemma upd_updN : forall ls (a : nat) v,
   (a < pow2 32)%nat
-  -> upd ls a v = updN ls a v.
+  -> upd ls (natToW a) v = updN ls a v.
   unfold upd; intros; rewrite wordToNat_natToWord_idempotent; auto.
 Qed.
 
